src/Sound/Data/Ast/Stmt.dfy
@@ -24,86 +24,83 @@ module AST {
       case _ => false
     }
 
-//     function Depth(): Idx {
-//       match this
-//       case InArgument(v) => v + 1
-//       case InOutArgument(v) => v + 1
-//       case OutArgument(v) => v + 1
-//     }
+    predicate IsDefinedOn(d: set<Variable>) {
+      {this.v} <= d
+    }
 
-//     predicate IsDefinedOn(d: Idx) {
-//       Depth() <= d
-//     }
-
-//     function Eval(s: State): M.Any
-//       requires IsDefinedOn(|s|)
-//     {
-//       match this
-//       case InArgument(v) => s[v]
-//       case InOutArgument(v) => s[v]
-//       case OutArgument(v) => s[v]
-//     }
+    function Eval(s: State): M.Any
+      requires IsDefinedOn(s.Keys)
+    {
+      match mode
+      case In => s[v]
+      case InOut => s[v]
+      case Out => s[v]
+    }
   }
 
   newtype CallArguments = seq<CallArgument> {
-
-    function Vars(): set<Variable> {
-      if this == [] then {} else {this[0].v} + this[1..].Vars()
-    }
 
     function OutArgs(): set<Variable> {
       if this == [] then {} else this[0].OutArg() + this[1..].OutArgs()
     }
 
-//     function InOutArgs(): seq<Idx> 
-//       ensures |InOutArgs()| == NumInOutArgs()
-//     {
-//       if this == [] then 
-//         [] else 
-//       if this[0].IsInOutArg() then 
-//         [this[0].v] + this[1..].InOutArgs() 
-//       else this[1..].InOutArgs()
-//     }
+    function NumInOutArgs(): nat {
+      if this == [] then 
+        0 
+      else 
+        if this[0].mode == InOut then 
+          1 + this[1..].NumInOutArgs() 
+        else this[1..].NumInOutArgs()
+    }
 
-//     lemma InOutArgsLemma(v: Idx)
-//       requires v in InOutArgs()
-//       ensures InOutArgument(v) in this
-//     {
 
-//     }
+    function InOutArgs(): seq<Variable> 
+      ensures |InOutArgs()| == NumInOutArgs()
+    {
+      if this == [] then 
+        [] else 
+      if this[0].IsInOutArg() then 
+        [this[0].v] + this[1..].InOutArgs() 
+      else this[1..].InOutArgs()
+    }
 
-//     lemma OutArgsDepthLemma()
-//       ensures forall v <- OutArgs() :: v < Depth()
-//     { }
+    lemma InOutArgsLemma(v: Variable)
+      requires v in InOutArgs()
+      ensures CallArgument(v, InOut) in this
+    {
 
-//     function Depth(): Idx {
-//       if this == [] then 0 else max(this[0].Depth(), this[1..].Depth())
-//     }
+    }
 
-//     predicate IsDefinedOn(d: Idx) {
-//       Depth() <= d
-//     }
+    lemma OutArgsDepthLemma()
+      ensures OutArgs() <= FVars()
+    { }
 
-//     lemma IsDefinedOnIn(arg: CallArgument, d: Idx)
-//       requires arg in this
-//       requires IsDefinedOn(d)
-//       ensures arg.IsDefinedOn(d)
-//     { 
-//       if this != [] {
-//         if arg != this[0] {
-//           this[1..].IsDefinedOnIn(arg, d);
-//         }
-//       }
-//     }
+    function FVars(): set<Variable> {
+      if this == [] then {} else {this[0].v} + this[1..].FVars()
+    }
+
+    predicate IsDefinedOn(d: set<Variable>) {
+      FVars() <= d
+    }
+
+    lemma IsDefinedOnIn(arg: CallArgument, d: set<Variable>)
+      requires arg in this
+      requires IsDefinedOn(d)
+      ensures arg.IsDefinedOn(d)
+    { 
+      if this != [] {
+        if arg != this[0] {
+          this[1..].IsDefinedOnIn(arg, d);
+        }
+      }
+    }
       
-//     function Eval(s: State): State 
-//       requires IsDefinedOn(|s|)
-//       ensures |Eval(s)| == |this|
-//     {
-//       seq(|this|, (i: nat) requires i < |this| => 
-//         IsDefinedOnIn(this[i], |s|);
-//         this[i].Eval(s))
-//     }
+    function Eval(s: State): State 
+      requires IsDefinedOn(s.Keys)
+      ensures Eval(s).Keys == FVars()
+    {
+      map v | v in FVars() :: s[v]
+    }
 
 //     function EvalOld(s: State): State 
 //       requires IsDefinedOn(|s|)
@@ -114,15 +111,6 @@ module AST {
 //         IsDefinedOnIn(InOutArgument(InOutArgs()[i]), |s|);
 //         s[InOutArgs()[i]]
 //       )
-//     }
-
-//     function NumInOutArgs(): nat {
-//       if this == [] then 
-//         0 
-//       else 
-//         if this[0].InOutArgument? then 
-//           1 + this[1..].NumInOutArgs() 
-//         else this[1..].NumInOutArgs()
 //     }
 
 //     lemma NumInOutArgsConcatLemma(args: CallArguments)
@@ -150,15 +138,15 @@ module AST {
       SetOfSeq(seq(|Parameters|, (i: nat) requires i < |Parameters| => Parameters[i].v))
     }
 
-//     function NumInOutArgs'(Parameters: seq<Parameter>): nat {
-//       if Parameters == [] then 0 else
-//       if Parameters[0].mode == InOut then 1 + NumInOutArgs'(Parameters[1..]) else
-//       NumInOutArgs'(Parameters[1..])
-//     }
+    function NumInOutArgs'(Parameters: seq<Parameter>): nat {
+      if Parameters == [] then 0 else
+      if Parameters[0].mode == InOut then 1 + NumInOutArgs'(Parameters[1..]) else
+      NumInOutArgs'(Parameters[1..])
+    }
 
-//     function NumInOutArgs(): nat {
-//       NumInOutArgs'(Parameters)
-//     }
+    function NumInOutArgs(): nat {
+      NumInOutArgs'(Parameters)
+    }
 
 //     predicate IsOldVar(i: Idx) 
 //     {
@@ -199,6 +187,7 @@ module AST {
       ensures SeqValidCalls(PostCheck'(p))
       ensures SeqIsDefinedOn(PostCheck'(p), ParametersKeys() /*+ NumInOutArgs()*/)
       ensures SeqJumpsDefinedOn(PostCheck'(p), 0)
+      ensures SeqVariablesDistinct(PostCheck'(p), ParametersKeys() /*+ NumInOutArgs()*/)
     {
       if p == [] then [] else
         assert forall e <- p[1..] :: e in p;
@@ -212,6 +201,7 @@ module AST {
       requires Valid()
       ensures SeqValidCalls(PostCheck())
       ensures SeqIsDefinedOn(PostCheck(), ParametersKeys() /*+ NumInOutArgs()*/)
+      ensures SeqVariablesDistinct(PostCheck(), ParametersKeys() /*+ NumInOutArgs()*/)
       reads this`Body
     {
       PostCheck'(Post)
@@ -251,7 +241,7 @@ module AST {
 //         st[InOutVarsIdxs()[i]])
 //     }
 
-    predicate ValidBody() 
+    ghost predicate ValidBody() 
       requires Body.Some?
       reads this`Body
     {
@@ -259,10 +249,11 @@ module AST {
       && body.ValidCalls()
       && body.IsDefinedOn(ParametersKeys() /*+ NumInOutArgs()*/)
       && body.JumpsDefinedOn(0)
+      && body.VariablesDistinct(ParametersKeys() /*+ NumInOutArgs()*/)
       // && body.ImmutableVars(OldVars())
     }
 
-    predicate Valid() 
+    ghost predicate Valid() 
       reads this`Body
     {
       && (Body.Some? ==> ValidBody())
@@ -282,10 +273,69 @@ module AST {
       if Body.Some? then Body.value.FunctionsCalled() + SeqExprFunctionsCalled(Pre) + SeqExprFunctionsCalled(Post) else {}
     }
 
+    ghost predicate IsSafe(m: M.Model) 
+      reads this`Body
+    {
+      && (forall e <- Pre :: e.IsSafe(m))
+      && (forall e <- Post :: e.IsSafe(m))
+      && (Body.Some? ==> Body.value.IsSafe(m))
+    }
+
+    lemma IsSafeLemma'(p: seq<Expr>, m: M.Model)
+      requires forall e <- p :: e.IsSafe(m)
+      requires forall e <- p :: e.IsDefinedOn(ParametersKeys() /*+ NumInOutArgs()*/)
+      ensures SeqIsSafe(PostCheck'(p), m)
+    {
+      if p != [] {
+        assert p[0] in p;
+        IsSafeLemma'(p[1..], m) by {
+          assert forall e <- p[1..] :: e in p;
+        }
+      }
+    }
+
+    lemma IsSafeLemma(m: M.Model)
+      requires IsSafe(m)
+      requires Valid()
+      ensures SeqIsSafe(PostCheck(), m)
+    {
+      IsSafeLemma'(Post, m);
+    }
+
+    ghost predicate IsSafeWith(funs: set<Function>)
+      reads *
+    {
+      forall md: M.Model ::
+        (forall func <- funs :: func.IsSound(md)) ==> IsSafe(md)
+    }
+
+    lemma IsSafePostCheckLemma'(m: M.Model, p: seq<Expr>)
+      requires forall e <- p :: e.IsSafe(m)
+      requires forall e <- p :: e.IsDefinedOn(ParametersKeys() /*+ NumInOutArgs()*/)
+      ensures SeqIsSafe(PostCheck'(p), m)
+    {
+      if p != [] {
+        assert p[0] in p;
+        IsSafePostCheckLemma'(m, p[1..]);
+      }
+    }
+
+    lemma IsSafePostCheckLemma(m: M.Model)
+      requires IsSafe(m)
+      requires Valid()
+      ensures SeqIsSafe(PostCheck(), m)
+    {
+      IsSafePostCheckLemma'(m, Post);
+    }
   }
 
+  ghost predicate SeqSafeWith(procs: seq<Procedure>, funs: set<Function>)
+    reads *
+  {
+    forall proc <- procs :: proc.IsSafeWith(funs)
+  }
 
-    datatype Stmt =
+  datatype Stmt =
     | Check(e: Expr)
     | Assume(e: Expr)
     | Seq(ss: seq<Stmt>)
@@ -306,11 +356,21 @@ module AST {
       case _ => false
     }
 
+    ghost predicate VariablesDistinct(vars: set<Variable>)
+    {
+      match this
+      case Seq(ss) => SeqVariablesDistinct(ss, vars)
+      case Choice(s0, s1) => s0.VariablesDistinct(vars) && s1.VariablesDistinct(vars)
+      case NewScope(vs, s) => vs !! vars && s.VariablesDistinct(vars + vs)
+      case Loop(inv, body) => body.VariablesDistinct(vars)
+      case _ => true
+    }
+
     predicate ValidCalls() {
       match this
       case Call(proc, args) =>
-        && (forall e <- proc.Pre :: e.IsDefinedOn(args.Vars()))
-        && (forall e <- proc.Post :: e.IsDefinedOn(args.Vars() /*+ args.NumInOutArgs()*/))
+        && SeqExprFVars(proc.Pre) <= args.FVars()
+        && SeqExprFVars(proc.Post) <= args.FVars() /*+ args.NumInOutArgs()*/
       case Seq(ss) => forall s <- ss :: s.ValidCalls()
       case Choice(s0, s1) => s0.ValidCalls() && s1.ValidCalls()
       case NewScope(n, s) => s.ValidCalls()
@@ -337,12 +397,21 @@ module AST {
       case Check(e) => e.FVars()
       case Assume(e) => e.FVars()
       case Seq(ss) => SeqFVars(ss)
-      case Assign(x, _) => {x}
+      case Assign(x, rhs) => {x} + rhs.FVars()
       case Choice(s0, s1) => s0.FVars() + s1.FVars()
       case NewScope(vars, s) => vars + s.FVars()
       case Escape(l) => {}
       case Loop(inv, body) => inv.FVars() + body.FVars()
-      case Call(proc, args) => args.Vars() /*+ args.NumInOutArgs()*/
+      case Call(proc, args) => args.FVars() /*+ args.NumInOutArgs()*/
+    }
+
+    function BVars(): set<Variable> {
+      match this
+      case Choice(s0, s1) => s0.BVars() + s1.BVars()
+      case NewScope(vars, s) => vars + s.BVars()
+      case Loop(inv, body) => body.BVars()
+      case Seq(ss) => SeqBVars(ss)
+      case _ => {}
     }
 
     predicate IsDefinedOn(vars: set<Variable>) 
@@ -391,6 +460,32 @@ module AST {
       case Escape(l) => {}
     }
 
+    lemma VariablesDistinctBVars(vs: set<Variable>)
+      requires VariablesDistinct(vs)
+      ensures vs !! BVars()
+    {
+      match this
+      case Seq(ss) => 
+        DistinctSeqBVars(ss, vs) by {
+          forall s | s in ss { s.VariablesDistinctBVars(vs); }
+        }
+      case _ => 
+    }
+
+    lemma VariablesDistinctUnion(vars1: set<Variable>, vars2: set<Variable>)
+      requires VariablesDistinct(vars1)
+      requires vars2 !! BVars()
+      ensures VariablesDistinct(vars1 + vars2)
+    {
+      match this
+      case Seq(ss) => SeqVariablesDistinctUnion(ss, vars1, vars2);
+      case NewScope(vars, s) => 
+        s.VariablesDistinctBVars(vars1 + vars);
+        s.VariablesDistinctUnion(vars1 + vars, vars2);
+        assert vars1 + vars + vars2 == vars1 + vars2 + vars;
+      case _ => 
+    }
+
 //     predicate ImmutableVarsIdx(vars: set<Idx>, i: Idx) {
 //       match this
 //       case Assign(x, _) => x + i !in vars
@@ -409,13 +504,127 @@ module AST {
       requires d1 <= d2
       ensures IsDefinedOn(d1) ==> IsDefinedOn(d2)
     {  }
+
+    ghost predicate IsSafe(m: M.Model) {
+      match this
+      case Check(e) => e.IsSafe(m)
+      case Assume(e) => e.IsSafe(m)
+      case Assign(_, e) => e.IsSafe(m)
+      case Seq(ss) => SeqIsSafe(ss, m)
+      case Choice(s0, s1) => s0.IsSafe(m) && s1.IsSafe(m)
+      case NewScope(_, s) => s.IsSafe(m)
+      case Escape(l) => true
+      case Loop(inv, body) => inv.IsSafe(m) && body.IsSafe(m)
+      case Call(proc, args) => true
+    }
+  }
+
+  ghost predicate SeqIsSafe(ss: seq<Stmt>, m: M.Model) {
+    forall s <- ss :: s.IsSafe(m)
+  }
+
+  lemma SeqIsSafeSeq(ss: seq<Stmt>, cont: seq<Stmt>, m: M.Model)
+    requires SeqIsSafe([Seq(ss)] + cont, m)
+    ensures SeqIsSafe(ss, m)
+  {
+    assert Seq(ss) in [Seq(ss)] + cont;
+  }
+
+  lemma ChoiceIsSafe(s1: Stmt, s2: Stmt, cont: seq<Stmt>, m: M.Model)
+    requires SeqIsSafe([Choice(s1, s2)] + cont, m)
+    ensures SeqIsSafe([s1] + cont, m)
+    ensures SeqIsSafe([s2] + cont, m)
+  {
+    assert Choice(s1, s2) in [Choice(s1, s2)] + cont;
+    assert Choice(s1, s2).IsSafe(m);
+  }
+
+  lemma NewScopeIsSafe(vars: set<Variable>, s: Stmt, cont: seq<Stmt>, m: M.Model)
+    requires SeqIsSafe([NewScope(vars, s)] + cont, m)
+    ensures SeqIsSafe([s], m)
+  {
+    assert NewScope(vars, s) in [NewScope(vars, s)] + cont;
+    assert NewScope(vars, s).IsSafe(m);
+  }
+
+  lemma LoopIsSafe(inv: Expr, body: Stmt, cont: seq<Stmt>, m: M.Model)
+    requires SeqIsSafe([Loop(inv, body)] + cont, m)
+    ensures SeqIsSafe([Assume(inv), body, Check(inv), Assume(BConst(false))], m)
+  {
+    assert Loop(inv, body) in [Loop(inv, body)] + cont;
+    assert Loop(inv, body).IsSafe(m);
+  }
+
+  ghost predicate SeqVariablesDistinct(ss: seq<Stmt>, vars: set<Variable>)
+  {
+    forall s <- ss :: s.VariablesDistinct(vars)
+  }
+
+  lemma SeqVariablesDistinctSeq(ss: seq<Stmt>, cont: seq<Stmt>, vars: set<Variable>)
+    requires SeqVariablesDistinct([Seq(ss)] + cont, vars)
+    ensures SeqVariablesDistinct(ss + cont, vars)
+  {
+    forall s | s in ss + cont ensures s.VariablesDistinct(vars) {
+      if s in cont {
+        assert s in [Seq(ss)] + cont;
+      } else {
+        assert Seq(ss) in [Seq(ss)] + cont;
+        assert SeqVariablesDistinct(ss, vars);
+      }
+    }
+  }
+
+  lemma SeqVariablesDistinctChoice(s1: Stmt, s2: Stmt, cont: seq<Stmt>, vars: set<Variable>)
+    requires SeqVariablesDistinct([Choice(s1, s2)] + cont, vars)
+    ensures SeqVariablesDistinct([s1] + cont, vars)
+    ensures SeqVariablesDistinct([s2] + cont, vars)
+  {
+    forall s | s in [s1] + [s2] + cont ensures s.VariablesDistinct(vars) {
+      if s in cont {
+        assert s in [Choice(s1, s2)] + cont;
+      } else if s == s1 || s == s2 {
+        assert Choice(s1, s2) in [Choice(s1, s2)] + cont;
+        assert Choice(s1, s2).VariablesDistinct(vars);
+      }
+    }
+  }
+
+
+
+  lemma SeqVariablesDistinctNewScope(s: Stmt, vars: set<Variable>, cont: seq<Stmt>, vs: set<Variable>)
+    requires SeqVariablesDistinct([NewScope(vars, s)] + cont, vs)
+    ensures SeqVariablesDistinct([s], vs + vars)
+    ensures vs + vars !! SeqBVars([s])
+  {
+    assert NewScope(vars, s) in [NewScope(vars, s)] + cont;
+    assert NewScope(vars, s).VariablesDistinct(vs);
+    s.VariablesDistinctBVars(vs + vars);
+  }
+
+  lemma SeqVariablesDistinctUnion(ss: seq<Stmt>, vars1: set<Variable>, vars2: set<Variable>)
+    requires SeqVariablesDistinct(ss, vars1)
+    requires vars2 !! SeqBVars(ss)
+    ensures SeqVariablesDistinct(ss, vars1 + vars2)
+  {
+    forall s | s in ss ensures s.VariablesDistinct(vars1 + vars2) {
+      DistinctSeqBVars'(ss, vars2, s);
+      s.VariablesDistinctUnion(vars1, vars2);
+    }
+  }
+
+  lemma SeqVariablesDistinctLoop(body: Stmt, inv: Expr, cont: seq<Stmt>, vars: set<Variable>)
+    requires SeqVariablesDistinct([Loop(inv, body)] + cont, vars)
+    ensures SeqVariablesDistinct([Assume(inv), body, Check(inv), Assume(BConst(false))], vars)
+  {
+    assert body.VariablesDistinct(vars) by {
+      assert Loop(inv, body) in [Loop(inv, body)] + cont;
+      assert Loop(inv, body).VariablesDistinct(vars);
+    }
   }
 
   predicate SeqValidCalls(ss: seq<Stmt>) {
     forall s <- ss :: s.ValidCalls()
   }
-
-//   // lemma SeqValidCallsLemma(ss: seq<Stmt>, s: Stmt)
 
   function SeqProceduresCalled(ss: seq<Stmt>): set<Procedure> {
     if ss == [] then {} else ss[0].ProceduresCalled() + SeqProceduresCalled(ss[1..])
@@ -453,10 +662,35 @@ module AST {
     if ss == [] then {} else ss[0].FVars() + SeqFVars(ss[1..])
   }
 
+  function SeqBVars(ss: seq<Stmt>): set<Variable> {
+    if ss == [] then {} else ss[0].BVars() + SeqBVars(ss[1..])
+  }
+
+  lemma DistinctSeqBVars(ss: seq<Stmt>, vars: set<Variable>)
+    requires forall s <- ss :: vars !! s.BVars()
+    ensures vars !! SeqBVars(ss)
+  {  }
+
+  lemma DistinctSeqBVars'(ss: seq<Stmt>, vars: set<Variable>, s: Stmt)
+    requires vars !! SeqBVars(ss)
+    requires s in ss
+    ensures vars !! s.BVars()
+  {  }
+
   predicate SeqIsDefinedOn(ss: seq<Stmt>, d: set<Variable>) 
     ensures SeqIsDefinedOn(ss, d) <==> SeqFVars(ss) <= d
   {
     if ss == [] then true else ss[0].IsDefinedOn(d) && SeqIsDefinedOn(ss[1..], d)
+  }
+
+  lemma SeqIsDefinedOnForall(ss: seq<Stmt>, d: set<Variable>)
+    requires forall s <- ss :: s.IsDefinedOn(d)
+    ensures SeqIsDefinedOn(ss, d)
+  {
+    // if ss != [] {
+    //   assert ss[0].IsDefinedOn(d);
+    //   assert SeqIsDefinedOn(ss[1..], d);
+    // }
   }
 
   function SeqJumpDepth(ss: seq<Stmt>): nat {
@@ -470,10 +704,9 @@ module AST {
   }
 
   lemma SeqFunConcatLemmas(ss1: seq<Stmt>, ss2: seq<Stmt>)
-    requires SeqValidCalls(ss1)
-    requires SeqValidCalls(ss2)
     ensures SeqSize(ss1 + ss2) == SeqSize(ss1) + SeqSize(ss2)
     ensures SeqFVars(ss1 + ss2) == SeqFVars(ss1) + SeqFVars(ss2)
+    ensures SeqBVars(ss1 + ss2) == SeqBVars(ss1) + SeqBVars(ss2)
     ensures SeqJumpDepth(ss1 + ss2) == max(SeqJumpDepth(ss1), SeqJumpDepth(ss2))
     ensures SeqFunctionsCalled(ss1 + ss2) == SeqFunctionsCalled(ss1) + SeqFunctionsCalled(ss2)
   {
