src/Sound/VCGen/BlockContinuation.dfy
@@ -1,220 +1,300 @@
-// module Block {
-//   import opened Utils
-//   import M = Model
-//   import opened Expr
-//   import opened AST
-//   import opened State
+module Block {
+  import opened Utils
+  import M = Model
+  import opened Expr
+  import opened AST
+  import opened State
 
-//   datatype Point = Point(cont: seq<Stmt>, varsInScope: nat)
+  datatype Point = Point(cont: seq<Stmt>, varsInScope: set<Variable>)
 
-//   newtype Continuation = seq<Point> {
+  newtype Continuation = seq<Point> {
 
-//     predicate ValidCalls() {
-//       forall p <- this :: SeqValidCalls(p.cont)
-//     }
+    ghost predicate IsSafe(md: M.Model) {
+      forall p <- this :: SeqIsSafe(p.cont, md)
+    }
 
-//     function FunctionsCalled(): set<Function> {
-//       if this == [] then {} else SeqFunctionsCalled(this[0].cont) + this[1..].FunctionsCalled()
-//     }
+    predicate ValidCalls() {
+      forall p <- this :: SeqValidCalls(p.cont)
+    }
 
-//     lemma FunctionsCalledSuffix(l: nat)
-//       requires l < |this|
-//       ensures this[l..].FunctionsCalled() <= FunctionsCalled()
-//     {
-//       if l != 0 {
-//         assert this[l..] == [this[l]] + this[l + 1..];
-//         // TODO: Might be a soundness bug
-//         FunctionsCalledSuffix(l - 1);
-//       }
-//     }
+    ghost opaque predicate VariablesDistinct(vars: set<Variable>) {
+      if this == [] then true else
+        && this[0].varsInScope <= vars
+        && SeqVariablesDistinct(this[0].cont, vars - this[0].varsInScope) 
+        && this[0].varsInScope !! this[1..].AllVarsInScope()
+        && this[1..].VariablesDistinct(vars - this[0].varsInScope)
+        // this[0].varsInScope !! vars && this[1..].VariablesDistinct(vars, this[0].varsInScope + bvars)
+    }
 
-//     function Update(cont: seq<Stmt>, varsInScope: nat): Continuation {
-//       [Point(cont, varsInScope)] + this
-//     }
 
-//     function VarsInScope(l: nat): nat 
-//       requires l <= |this|
-//     {
-//       if l == 0 then 0 else this[0].varsInScope + this[1..].VarsInScope(l - 1)
-//     }
+    function FunctionsCalled(): set<Function> {
+      if this == [] then {} else SeqFunctionsCalled(this[0].cont) + this[1..].FunctionsCalled()
+    }
 
-//     function AllVarsInScope(): nat {
-//       if this == [] then 0 else this[0].varsInScope + this[1..].AllVarsInScope()
-//     }
+    lemma FunctionsCalledSuffix(l: nat)
+      requires l < |this|
+      ensures this[l..].FunctionsCalled() <= FunctionsCalled()
+    {
+      if l != 0 {
+        assert this[l..] == [this[l]] + this[l + 1..];
+        // TODO: Might be a soundness bug
+        FunctionsCalledSuffix(l - 1);
+      }
+    }
 
-//     lemma VarsInScopeLeqAll(l: nat)
-//       requires l <= |this|
-//       ensures VarsInScope(l) + this[l..].AllVarsInScope() == AllVarsInScope()
-//     {
+    function Update(cont: seq<Stmt>, varsInScope: set<Variable>): Continuation {
+      [Point(cont, varsInScope as set<Variable>)] + this
+    }
 
-//     }
+    function VarsInScope(l: nat): set<Variable> 
+      requires l <= |this|
+    {
+      if l == 0 then {} else this[0].varsInScope + this[1..].VarsInScope(l - 1)
+    }
 
-//     lemma VarsInScopeSuffix(l: nat)
-//       requires l <= |this|
-//       ensures VarsInScope(l) == this[..l].AllVarsInScope()
-//     {
-//       if l != 0 {
-//         calc {
-//           VarsInScope(l);
-//         ==
-//           this[0].varsInScope + this[1..].VarsInScope(l - 1);
-//         == { this[1..].VarsInScopeSuffix(l - 1);
-//              assert this[1..][..l - 1] == this[1..l]; }
-//           this[0].varsInScope + this[1..l].AllVarsInScope();
-//         == { assert this[..l][1..] == this[1..l]; }
-//           this[..l].AllVarsInScope();
-//         }
+    function AllVarsInScope(): set<Variable> {
+      if this == [] then {} else this[0].varsInScope + this[1..].AllVarsInScope()
+    }
 
-//       }
-//     }
+    lemma VarsInScopeLeqAll(l: nat)
+      requires l <= |this|
+      ensures VarsInScope(l) + this[l..].AllVarsInScope() == AllVarsInScope()
+    {
 
-//     function Size(): nat {
-//       if this == [] then 0 else SeqSize(this[0].cont) + 1 + this[1..].Size()
-//     }
+    }
 
-//     lemma UpdateSize(cont: seq<Stmt>, varsInScope: nat)
-//       ensures Update(cont, varsInScope).Size() == SeqSize(cont) + Size() + 1
-//     {
+    lemma VarsInScopeSuffix(l: nat)
+      requires l <= |this|
+      ensures VarsInScope(l) == this[..l].AllVarsInScope()
+    {
+      if l != 0 {
+        calc {
+          VarsInScope(l);
+        ==
+          this[0].varsInScope + this[1..].VarsInScope(l - 1);
+        == { this[1..].VarsInScopeSuffix(l - 1);
+             assert this[1..][..l - 1] == this[1..l]; }
+          this[0].varsInScope + this[1..l].AllVarsInScope();
+        == { assert this[..l][1..] == this[1..l]; }
+          this[..l].AllVarsInScope();
+        }
 
-//     }
+      }
+    }
 
-//     lemma SizePrefix(l: nat)
-//       requires l <= |this|
-//       ensures this[l..].Size() <= Size()
-//     {
-//       assert this[..l] + this[l..] == this;
-//       SizeConcat(this[..l], this[l..]);
-//     }
+    function Size(): nat {
+      if this == [] then 0 else SeqSize(this[0].cont) + 1 + this[1..].Size()
+    }
 
-//     predicate IsDefinedOn(d: nat) {
-//       AllVarsInScope() <= d
-//     }
+    lemma UpdateSize(cont: seq<Stmt>, varsInScope: set<Variable>)
+      ensures Update(cont, varsInScope).Size() == SeqSize(cont) + Size() + 1
+    {
 
-//     predicate JumpsDefined() {
-//       if this == [] then true else
-//         SeqJumpsDefinedOn(this[0].cont, |this[1..]|) && this[1..].JumpsDefined()
-//     }
+    }
 
-//     predicate VarsDefined(n: nat) 
-//       requires ValidCalls()
-//       requires IsDefinedOn(n)
-//     {
-//       if this == [] then true else
-//         SeqIsDefinedOn(this[0].cont, n - this[0].varsInScope) && this[1..].VarsDefined(n - this[0].varsInScope)
-//     }
+    lemma SizePrefix(l: nat)
+      requires l <= |this|
+      ensures this[l..].Size() <= Size()
+    {
+      assert this[..l] + this[l..] == this;
+      SizeConcat(this[..l], this[l..]);
+    }
 
-//     lemma VarsDefinedTransitivity(n1: nat, n2: nat)
-//       requires ValidCalls()
-//       requires IsDefinedOn(n1)
-//       requires VarsDefined(n1)
-//       requires n1 <= n2
-//       ensures VarsDefined(n2)
-//     {
+    predicate IsDefinedOn(d: set<Variable>) {
+      AllVarsInScope() <= d
+    }
 
-//     }
+    predicate JumpsDefined() {
+      if this == [] then true else
+        SeqJumpsDefinedOn(this[0].cont, |this[1..]|) && this[1..].JumpsDefined()
+    }
 
-//     lemma AllVarsInScopeSuffixSucc(l: nat)
-//       requires l < |this|
-//       ensures this[..l + 1].AllVarsInScope() == this[..l].AllVarsInScope() + this[l].varsInScope
-//       // ensures AllVarsInScope() == this[..l + 1].AllVarsInScope()
-//     {
-//       VarsInScopeSuffix(l);
-//       VarsInScopeLeqAll(l);
-//       VarsInScopeLeqAll(l + 1);
-//       VarsInScopeSuffix(l + 1);
-//     }
+    predicate VarsDefined(vars: set<Variable>) 
+      requires ValidCalls()
+      // requires IsDefinedOn(vars)
+    {
+      if this == [] then true else
+        && SeqIsDefinedOn(this[0].cont, vars - this[0].varsInScope) 
+        && this[1..].VarsDefined(vars - this[0].varsInScope)
+    }
 
-//     lemma DefinedPrefix''(l: nat, n: nat)
-//       requires l <= |this|
-//       requires ValidCalls()
-//       requires IsDefinedOn(n)
-//       ensures n >= this[..l].AllVarsInScope()
-//     {
-//       VarsInScopeSuffix(l);
-//       VarsInScopeLeqAll(l);
-//     }
+    lemma VarsDefinedTransitivity(vars1: set<Variable>, vars2: set<Variable>)
+      requires ValidCalls()
+      // requires IsDefinedOn(vars1)
+      requires VarsDefined(vars1)
+      requires vars1 <= vars2
+      ensures VarsDefined(vars2)
+    {
+      if this != [] {
+        this[1..].VarsDefinedTransitivity(vars1 - this[0].varsInScope, vars2 - this[0].varsInScope);
+      }
+    }
 
-//     lemma DefinedPrefix'(l: nat, n: nat)
-//       requires l < |this|
-//       requires ValidCalls()
-//       requires JumpsDefined()
-//       requires IsDefinedOn(n)
-//       requires VarsDefined(n)
-//       ensures SeqJumpsDefinedOn(this[l].cont, |this[l + 1..]|) 
-//       ensures n >= this[..l + 1].AllVarsInScope()
-//       ensures SeqIsDefinedOn(this[l].cont, n - this[..l + 1].AllVarsInScope())
-//       // ensures SeqIsDefinedOn(this[l].cont, 1000) /*SOUNDNESS BUG:*/
-//     {
-//       DefinedPrefix''(l + 1, n);
-//       if this != [] {
-//         if l != 0 {
-//           assert this[1..][l - 1] == this[l];
-//           assert this[1..][l - 1..] == this[l..];
-//           assert this[1..][..l] == this[1..l + 1];
-//           this[1..].DefinedPrefix'(l - 1, n - this[0].varsInScope);
-//           assert SeqIsDefinedOn(this[l].cont, n - this[0].varsInScope - this[1..l + 1].AllVarsInScope());
-//           assert SeqIsDefinedOn(this[l].cont, n - this[..l + 1].AllVarsInScope());
-//         }
-//       }
-//     }
+    lemma AllVarsInScopeSuffixSucc(l: nat)
+      requires l < |this|
+      ensures this[..l + 1].AllVarsInScope() == this[..l].AllVarsInScope() + this[l].varsInScope
+      // ensures AllVarsInScope() == this[..l + 1].AllVarsInScope()
+    {
+      calc {
+        this[..l + 1].AllVarsInScope();
+        == { this[..l + 1].VarsInScopeLeqAll(l); }
+        this[..l + 1][l..].AllVarsInScope() + this[..l + 1].VarsInScope(l);
+        == { assert this[..l + 1][l..] == [this[l]]; }
+        this[l].varsInScope + this[..l + 1].VarsInScope(l);
+        == { this[..l + 1].VarsInScopeSuffix(l); }
+        this[l].varsInScope + this[..l + 1][..l].AllVarsInScope();
+        == { assert this[..l + 1][..l] == this[..l]; }
+        this[..l].AllVarsInScope() + this[l].varsInScope;
+      }
+    }
 
-//     lemma DefinedPrefix(l: nat, n: nat)
-//       requires l <= |this|
-//       requires ValidCalls()
-//       requires JumpsDefined()
-//       requires IsDefinedOn(n)
-//       requires VarsDefined(n)
-//       ensures this[l..].JumpsDefined()
-//       ensures n >= this[..l].AllVarsInScope()
-//       ensures this[l..].IsDefinedOn(n - this[..l].AllVarsInScope())
-//       ensures this[l..].VarsDefined(n - this[..l].AllVarsInScope())
-//       decreases |this| - l
-//     {
-//       if l != 0 {
-//         if |this| != l {
-//           assert this[l + 1..] == this[l..][1..];
-//           assert this[1..][..l - 1] == this[1..l];
-//           assert this[1..][..l] == this[1..l + 1];
-//           assert this[l..][0] == this[l];
-//           DefinedPrefix(l + 1, n);
-//           DefinedPrefix'(l, n);
-//           assert n >= this[..l+1].AllVarsInScope();
-//           assert this[..l+1].AllVarsInScope() == this[..l].AllVarsInScope() + this[l].varsInScope by {
-//             AllVarsInScopeSuffixSucc(l);
-//           }
-//           calc {
-//             this[l..].IsDefinedOn(n - this[..l].AllVarsInScope());
-//             { VarsInScopeLeqAll(l + 1); }
-//             SeqIsDefinedOn(this[l].cont, n - this[..l].AllVarsInScope()) && 
-//               this[l+1..].IsDefinedOn(n - this[..l].AllVarsInScope() - this[l].varsInScope);
-//             true;
-//           }
-//           var m := n - this[..l].AllVarsInScope();
-//           calc {
-//             this[l..].VarsDefined(m);
-//             SeqIsDefinedOn(this[l].cont, n - this[..l + 1].AllVarsInScope()) && 
-//             this[l + 1..].VarsDefined(n - this[..l + 1].AllVarsInScope());
-//             SeqIsDefinedOn(this[l].cont, n - this[..l + 1].AllVarsInScope());
-//             true;
-//           }
-//         } else {
-//           VarsInScopeLeqAll(|this|);
-//           VarsInScopeSuffix(|this|);
-//         }
-//       }
-//     }
-//   }
+    // lemma DefinedPrefix''(l: nat, vars: set<Variable>)
+    //   requires l <= |this|
+    //   requires ValidCalls()
+    //   // requires IsDefinedOn(vars)
+    //   ensures this[..l].AllVarsInScope() <= vars
+    // {
+    //   VarsInScopeSuffix(l);
+    //   VarsInScopeLeqAll(l);
+    // }
 
-//     lemma SizeConcat(cont1: Continuation, cont2: Continuation)
-//       ensures (cont1 + cont2).Size() == cont1.Size() + cont2.Size()
-//     {
-//       if cont1 == [] {
-//         assert cont1 + cont2 == cont2;
-//       } else {
-//         assert (cont1 + cont2)[0] == cont1[0];
-//         assert (cont1 + cont2)[1..] == cont1[1..] + cont2;
-//         SizeConcat(cont1[1..], cont2);
-//       }
-//     }
+    lemma VariablesDistinctPrefix(vars: set<Variable>, l: nat)
+      requires l <= |this|
+      requires VariablesDistinct(vars)
+      requires IsDefinedOn(vars)
+      ensures this[l..].VariablesDistinct(vars - VarsInScope(l))
+      ensures this[l..].AllVarsInScope() <= vars - VarsInScope(l)
+    {
+      if this != [] && l != 0 {
+        calc {
+          VariablesDistinct(vars);
+          ==> { reveal VariablesDistinct; }
+          && this[1..].VariablesDistinct(vars - this[0].varsInScope)
+          && this[0].varsInScope <= vars;
+          ==> { VariablesDistinctDisjoint(vars, 0);
+                this[1..].VariablesDistinctPrefix(vars - this[0].varsInScope, l - 1); }
+          && this[l..].VariablesDistinct(vars - this[0].varsInScope - this[1..].VarsInScope(l-1))
+          && this[l..].AllVarsInScope() <= vars - this[0].varsInScope - this[1..].VarsInScope(l-1);
+          == { assert vars - this[0].varsInScope - this[1..].VarsInScope(l-1) == 
+                      vars - (this[0].varsInScope + this[1..].VarsInScope(l-1)); }
+          && this[l..].VariablesDistinct(vars - VarsInScope(l))
+          && this[l..].AllVarsInScope() <= vars - VarsInScope(l);
+        }
+      } else {
+        assert vars - {} == vars;
+      }
+    }
 
-// }
+    lemma VariablesDistinctDisjoint(vars: set<Variable>, l: nat)
+      requires |this| > l
+      requires VariablesDistinct(vars)
+      ensures this[l].varsInScope !! this[l + 1..].AllVarsInScope()
+      ensures SeqVariablesDistinct(this[l].cont, vars - VarsInScope(l + 1))
+    {
+      if l != 0 {
+        calc {
+          VariablesDistinct(vars);
+          ==> { reveal VariablesDistinct; }
+          && this[1..].VariablesDistinct(vars - this[0].varsInScope);
+          ==> { this[1..].VariablesDistinctDisjoint(vars - this[0].varsInScope, l - 1); }
+          && this[l].varsInScope !! this[l+1..].AllVarsInScope()
+          && SeqVariablesDistinct(this[l].cont, vars - this[0].varsInScope - this[1..].VarsInScope(l));
+          == { assert vars - this[0].varsInScope - this[1..].VarsInScope(l) == 
+                      vars - (this[0].varsInScope + this[1..].VarsInScope(l)); }
+          && this[l].varsInScope !! this[l+1..].AllVarsInScope()
+          && SeqVariablesDistinct(this[l].cont, vars - VarsInScope(l + 1));
+        }
+      } else {
+        reveal VariablesDistinct;
+        assert VarsInScope(1) == this[0].varsInScope;
+      }
+    }
+
+    lemma DefinedPrefix'(l: nat, vars: set<Variable>)
+      requires l < |this|
+      requires ValidCalls()
+      requires JumpsDefined()
+      // requires VariablesDistinct(bvars)
+      // requires IsDefinedOn(vars)
+      requires VarsDefined(vars)
+      ensures SeqJumpsDefinedOn(this[l].cont, |this[l + 1..]|) 
+      // ensures this[..l + 1].AllVarsInScope() <= vars
+      ensures SeqIsDefinedOn(this[l].cont, vars - this[..l + 1].AllVarsInScope())
+      // ensures SeqIsDefinedOn(this[l].cont, 1000) /*SOUNDNESS BUG:*/
+    {
+      // DefinedPrefix''(l + 1, vars);
+      if this != [] {
+        if l != 0 {
+          assert this[1..][l - 1] == this[l];
+          assert this[1..][l - 1..] == this[l..];
+          assert this[1..][..l] == this[1..l + 1];
+          this[1..].DefinedPrefix'(l - 1, vars - this[0].varsInScope);
+          assert SeqIsDefinedOn(this[l].cont, vars - this[0].varsInScope - this[1..l + 1].AllVarsInScope());
+          assert SeqIsDefinedOn(this[l].cont, vars - this[..l + 1].AllVarsInScope());
+        }
+      }
+    }
+
+    lemma DefinedPrefix(l: nat, vars: set<Variable>)
+      requires l <= |this|
+      requires ValidCalls()
+      requires JumpsDefined()
+      // requires IsDefinedOn(vars)
+      requires VarsDefined(vars)
+      ensures this[l..].JumpsDefined()
+      // ensures this[..l].AllVarsInScope() <= vars
+      // ensures this[l..].IsDefinedOn(vars - this[..l].AllVarsInScope())
+      ensures this[l..].VarsDefined(vars - this[..l].AllVarsInScope())
+      decreases |this| - l
+    {
+      if l != 0 {
+        if |this| != l {
+          assert this[l + 1..] == this[l..][1..];
+          assert this[1..][..l - 1] == this[1..l];
+          assert this[1..][..l] == this[1..l + 1];
+          assert this[l..][0] == this[l];
+          DefinedPrefix(l + 1, vars);
+          DefinedPrefix'(l, vars);
+          // assert this[..l+1].AllVarsInScope() <= vars;
+          assert this[..l+1].AllVarsInScope() == this[..l].AllVarsInScope() + this[l].varsInScope by {
+            AllVarsInScopeSuffixSucc(l);
+          }
+          // calc {
+          //   this[l..].IsDefinedOn(vars - this[..l].AllVarsInScope());
+          //   { VarsInScopeLeqAll(l + 1); }
+          //   SeqIsDefinedOn(this[l].cont, vars - this[..l].AllVarsInScope()) && 
+          //     this[l+1..].IsDefinedOn(vars - this[..l].AllVarsInScope() - this[l].varsInScope);
+          //   true;
+          // }
+          var m := vars - this[..l].AllVarsInScope();
+          calc {
+            this[l..].VarsDefined(m);
+            { assert m - this[l].varsInScope == vars - this[..l + 1].AllVarsInScope(); }
+            SeqIsDefinedOn(this[l].cont, vars - this[..l + 1].AllVarsInScope()) && 
+            this[l + 1..].VarsDefined(vars - this[..l + 1].AllVarsInScope());
+            SeqIsDefinedOn(this[l].cont, vars - this[..l + 1].AllVarsInScope());
+            true;
+          }
+        } else {
+          VarsInScopeLeqAll(|this|);
+          VarsInScopeSuffix(|this|);
+        }
+      } else {
+        assert vars - this[..0].AllVarsInScope() == vars;
+      }
+    }
+  }
+
+    lemma SizeConcat(cont1: Continuation, cont2: Continuation)
+      ensures (cont1 + cont2).Size() == cont1.Size() + cont2.Size()
+    {
+      if cont1 == [] {
+        assert cont1 + cont2 == cont2;
+      } else {
+        assert (cont1 + cont2)[0] == cont1[0];
+        assert (cont1 + cont2)[1..] == cont1[1..] + cont2;
+        SizeConcat(cont1[1..], cont2);
+      }
+    }
+
+}
