src/Sound/VCGen/Context.dfy
@@ -9,13 +9,13 @@ module Context {
     ctx: seq<Expr>,
     incarnation: map<Variable, Variable>) 
   {
-    // ghost function Models(md: M.Model) : iset<State> { iset st: State | IsSatisfiedOn(st, md) }
+    ghost function Models(md: M.Model) : iset<State> { iset st: State | IsSatisfiedOn(st, md) }
 
-    // ghost function AdjustedModels(md: M.Model) : iset<State> { 
-    //   iset st: State | exists st' <- Models(md) {:InAdjustedModelsLemma(st', md)} :: AdjustState(st') == st
-    // }
+    ghost function AdjustedModels(md: M.Model) : iset<State> { 
+      iset st: State | exists st' <- Models(md) {:InAdjustedModelsLemma(st', md)} :: AdjustState(st') == st
+    }
 
-//     lemma InAdjustedModelsLemma(st: State, st': State, md: M.Model)
+    lemma InAdjustedModelsLemma(st: State, st': State, md: M.Model)
 //       requires IsSatisfiedOn(st', md)
 //       requires st == AdjustState(st')
 //       ensures st in AdjustedModels(md)
@@ -28,12 +28,21 @@ module Context {
       SeqExprFVars(ctx) + incarnation.Values
     }
 
+    function FreshVarSet(typ: Type, vars: set<Variable>): Variable
+      ensures FreshVarSet(typ, vars) !in incarnation.Values
+      ensures FreshVarSet(typ, vars) !in SeqExprFVars(ctx)
+      ensures FreshVarSet(typ, vars) !in vars
+      ensures forall c <- ctx :: FreshVarSet(typ, vars) !in c.FVars()
+      ensures FreshVarSet(typ, vars).typ == typ
+
     function FreshVar(typ: Type): Variable
-      ensures FreshVar(typ) !in incarnation
+      ensures FreshVar(typ) !in incarnation.Values
       ensures FreshVar(typ) !in SeqExprFVars(ctx)
       ensures forall c <- ctx :: FreshVar(typ) !in c.FVars()
       ensures FreshVar(typ).typ == typ
-    // TODO: implemet
+    {
+      FreshVarSet(typ, {})
+    }
 
     function AdjustState(s: State): State
       requires incarnation.Values <= s.Keys
@@ -48,55 +57,43 @@ module Context {
         s[incarnation[v]]
     }
 
-    function DeleteVar(vars: set<Variable>): Context
+    function UpdateIncarnation(v: Variable, x: Variable): Context
     {
-      Context(ctx, incarnation - vars)
+      Context(ctx, incarnation[v := x])
     }
 
-    lemma DeleteVarUnion(vars1: set<Variable>, vars2: set<Variable>)
-      ensures DeleteVar(vars1 + vars2) == DeleteVar(vars1).DeleteVar(vars2)
-    {
-    }
+    /*
+      incr = map[u -> v]
 
-    lemma DeleteEmpty()
-      ensures DeleteVar({}) == this
-    {
+      let v := .. in v + u
+    */
 
-    }
-
-    function SubstituteBVars(e: Expr, bVars: set<Variable>): Expr
-      requires e.IsDefinedOn(incarnation.Keys + bVars)
-      requires incarnation.Keys !! bVars
+    function Substitute(e: Expr): Expr
+      requires e.IsDefinedOn(incarnation.Keys)
       decreases e
     {
       match e
       case BConst(bvalue) => e
       case IConst(ivalue) => e
       case CustomConst(value) => e
-      case BVar(v) => if v in bVars then BVar(v) else BVar(incarnation[v])
-      case OperatorExpr(op, args) => OperatorExpr(op, SeqSubstituteBVars(args, bVars))
-      case FunctionCallExpr(func, args) => FunctionCallExpr(func, SeqSubstituteBVars(args, bVars))
+      case BVar(v) => BVar(incarnation[v])
+      case OperatorExpr(op, args) => OperatorExpr(op, SeqSubstitute(args))
+      case FunctionCallExpr(func, args) => FunctionCallExpr(func, SeqSubstitute(args))
       case LetExpr(v, rhs, body) => 
-        assert body.FVars() <= e.FVars() + {v};
-        LetExpr(v, SubstituteBVars(rhs, bVars), DeleteVar({v}).SubstituteBVars(body, bVars + {v}))
+        var v' := v.FreshVar(incarnation.Values);
+        LetExpr(v', Substitute(rhs), UpdateIncarnation(v, v').Substitute(body))
       case QuantifierExpr(univ, v, body) => 
-        assert body.FVars() <= e.FVars() + {v};
-        QuantifierExpr(univ, v, DeleteVar({v}).SubstituteBVars(body, bVars + {v}))
+        var v' := v.FreshVar(incarnation.Values);
+        QuantifierExpr(univ, v', UpdateIncarnation(v, v').Substitute(body))
     }
 
-    function SeqSubstituteBVars(ss: seq<Expr>, bVars: set<Variable>): seq<Expr>
-      requires SeqExprFVars(ss) <= incarnation.Keys + bVars
-      requires incarnation.Keys !! bVars
+    function SeqSubstitute(ss: seq<Expr>): seq<Expr>
+      requires SeqExprFVars(ss) <= incarnation.Keys
+      ensures |SeqSubstitute(ss)| == |ss|
       decreases ss
     {
       if ss == [] then [] else
-      [SubstituteBVars(ss[0], bVars)] + SeqSubstituteBVars(ss[1..], bVars)
-    }
-
-    function Substitute(e: Expr): Expr
-      requires e.IsDefinedOn(incarnation.Keys)
-    {
-      SubstituteBVars(e, {})
+      [Substitute(ss[0])] + SeqSubstitute(ss[1..])
     }
 
     function MkEntailment(e: Expr): Expr
@@ -106,16 +103,20 @@ module Context {
     }
 
     function MkEntailmentSeq(ss: seq<Expr>): seq<Expr>
-      requires forall e <- ss :: e.IsDefinedOn(incarnation.Keys)
+      requires SeqExprFVars(ss) <= incarnation.Keys
     {
-      seq(|ss|, (i: nat) requires i < |ss| => MkEntailment(ss[i]))
+      seq(|ss|, (i: nat) requires i < |ss| => 
+        SeqExprFVarsLemma(ss, ss[i]);
+        MkEntailment(ss[i]))
     }
 
     lemma MkEntailmentSeqLemma(ss: seq<Expr>, e: Expr)
-      requires forall e <- ss :: e.IsDefinedOn(incarnation.Keys)
+      requires SeqExprFVars(ss) <= incarnation.Keys
       requires e in ss
+      ensures forall e <- ss :: e.IsDefinedOn(incarnation.Keys)
       ensures MkEntailment(e) in MkEntailmentSeq(ss)
     {
+      forall e <- ss { SeqExprFVarsLemma(ss, e); }
       assert MkEntailment(e) == MkEntailmentSeq(ss)[Index(ss, e)];
     }
 
@@ -125,12 +126,7 @@ module Context {
     }
 
     /*
-
-    x -> y 
-
-    x && forall y, y
-
-    y -> 0
+    
     */
     ghost predicate IsSatisfiedOn(s: State, md: M.Model) 
     {
@@ -139,65 +135,51 @@ module Context {
       && (forall e <- ctx :: e.HoldsOn(s, md))
     }
 
-    lemma SubstituteBVarsIsDefinedOnLemma(e: Expr, bVars: set<Variable>, d: set<Variable>)
-      requires e.IsDefinedOn(incarnation.Keys + bVars)
+    lemma  SubstituteIsDefinedOnLemma(e: Expr, d: set<Variable>)
+      requires e.IsDefinedOn(incarnation.Keys)
       requires incarnation.Values <= d
-      requires bVars <= d
-      requires incarnation.Keys !! bVars
-      ensures SubstituteBVars(e, bVars).FVars() <= d
+      ensures Substitute(e).IsDefinedOn(d)
       decreases e
     {
-      match e 
-      case BVar(v) => if v !in bVars { 
-          assert v in incarnation.Keys;
-          assert incarnation[v] in incarnation.Values; 
-        }
-      case OperatorExpr(op, args) => 
-        SeqSubstituteBVarsIsDefinedOnLemma(args, bVars, d);
-      case QuantifierExpr(univ, v, body) =>
-        calc {        
-          SubstituteBVars(e, bVars).FVars();
-          == { assert body.FVars() <= e.FVars() + {v}; }
-          DeleteVar({v}).SubstituteBVars(body, bVars + {v}).FVars() - {v};
-          <= { DeleteVar({v}).SubstituteBVarsIsDefinedOnLemma(body, bVars + {v}, d + {v}); }
-          d;
-        }
+      match e
+      case BVar(v) => 
+        if v in incarnation.Keys { assert incarnation[v] in incarnation.Values; }
+      case OperatorExpr(op, args) =>
+        SeqSubstituteIsDefinedOnLemma(args, d);
       case FunctionCallExpr(func, args) =>
-        SeqSubstituteBVarsIsDefinedOnLemma(args, bVars, d);
+        SeqSubstituteIsDefinedOnLemma(args, d);
       case LetExpr(v, rhs, body) =>
-        calc {        
-          SubstituteBVars(e, bVars).FVars();
-          == { assert body.FVars() <= e.FVars() + {v}; }
-          SubstituteBVars(rhs, bVars).FVars() + 
-          (DeleteVar({v}).SubstituteBVars(body, bVars + {v}).FVars() - {v});
-          <= { DeleteVar({v}).SubstituteBVarsIsDefinedOnLemma(body, bVars + {v}, d + {v}); }
+        var v' := v.FreshVar(incarnation.Values);
+        calc {
+          Substitute(e).FVars();
+          == 
+          Substitute(rhs).FVars() + (UpdateIncarnation(v, v').Substitute(body).FVars() - {v'});
+          <= { UpdateIncarnation(v, v').SubstituteIsDefinedOnLemma(body, d + {v'}); }
+          d + (d + {v'} - {v'});
+        }
+      case QuantifierExpr(univ, v, body) =>
+        var v' := v.FreshVar(incarnation.Values);
+        calc {
+          Substitute(e).FVars();
+          == 
+          UpdateIncarnation(v, v').Substitute(body).FVars() - {v'};
+          <= { UpdateIncarnation(v, v').SubstituteIsDefinedOnLemma(body, d + {v'}); }
           d;
         }
       case _ =>
     }
 
-    lemma SeqSubstituteBVarsIsDefinedOnLemma(ss: seq<Expr>, bVars: set<Variable>, d: set<Variable>)
-      requires SeqExprFVars(ss) <= incarnation.Keys + bVars
+    lemma SeqSubstituteIsDefinedOnLemma(ss: seq<Expr>, d: set<Variable>)
+      requires SeqExprFVars(ss) <= incarnation.Keys
       requires incarnation.Values <= d
-      requires incarnation.Keys !! bVars
-      requires bVars <= d
-      ensures forall e <- SeqSubstituteBVars(ss, bVars) :: e.IsDefinedOn(d)
-      ensures SeqExprFVars(SeqSubstituteBVars(ss, bVars)) <= d
+      ensures forall e <- SeqSubstitute(ss) :: e.IsDefinedOn(d)
+      ensures SeqExprFVars(SeqSubstitute(ss)) <= d
       decreases ss
     {
       if ss != [] {
-        SubstituteBVarsIsDefinedOnLemma(ss[0], bVars, d);
-        SeqSubstituteBVarsIsDefinedOnLemma(ss[1..], bVars, d);
+        SubstituteIsDefinedOnLemma(ss[0], d);
+        SeqSubstituteIsDefinedOnLemma(ss[1..], d);
       }
-    }
-
-    lemma SubstituteIsDefinedOnLemma(e: Expr, d: set<Variable>)
-      requires e.IsDefinedOn(incarnation.Keys)
-      requires incarnation.Values <= d
-      ensures Substitute(e).FVars() <= d
-    {
-      DeleteEmpty();
-      SubstituteBVarsIsDefinedOnLemma(e, {}, d);
     }
 
     lemma ForallPush(s1: State, s2: State, e1: Expr, e2: Expr, v: Variable, md: M.Model)
@@ -205,6 +187,7 @@ module Context {
       requires e2.IsDefinedOn(s2.Keys + {v})
       requires forall b: M.Any | md.HasType(b, v.typ.ToType()) :: e1.Eval(s1.UpdateAt(v, b), md) == e2.Eval(s2.UpdateAt(v, b), md)
       ensures (forall b: M.Any | md.HasType(b, v.typ.ToType()) :: e1.HoldsOn(s1.UpdateAt(v, b), md)) == (forall b: M.Any | md.HasType(b, v.typ.ToType()) :: e2.HoldsOn(s2.UpdateAt(v, b), md))
+      ensures (forall b: M.Any | md.HasType(b, v.typ.ToType()) :: SomeBVal?(e1.Eval(s1.UpdateAt(v, b), md), md)) == (forall b: M.Any | md.HasType(b, v.typ.ToType()) :: SomeBVal?(e2.Eval(s2.UpdateAt(v, b), md), md))
     {  }
 
     lemma ExistsPush(s1: State, s2: State, e1: Expr, e2: Expr, v: Variable, md: M.Model)
@@ -214,115 +197,71 @@ module Context {
       ensures (exists b: M.Any | md.HasType(b, v.typ.ToType()) :: e1.HoldsOn(s1.UpdateAt(v, b), md)) == (exists b: M.Any | md.HasType(b, v.typ.ToType()) :: e2.HoldsOn(s2.UpdateAt(v, b), md))
     {  }
 
-    lemma SeqAdjustStateSubstituteBVarsLemma(ss: seq<Expr>, s: State, bVars: set<Variable>, md: M.Model)
-      requires SeqExprFVars(ss) <= incarnation.Keys + bVars
+    lemma SeqAdjustStateSubstituteLemma(ss: seq<Expr>, s: State, md: M.Model)
+      requires SeqExprFVars(ss) <= incarnation.Keys
       requires incarnation.Values <= s.Keys
-      requires bVars <= s.Keys
-      requires incarnation.Keys !! bVars
       ensures
-        (SeqSubstituteBVarsIsDefinedOnLemma(ss, bVars, s.Keys);
-         SeqEval(ss, s.Restrict(bVars) + AdjustStateBVars(s, bVars), md) == 
-         SeqEval(SeqSubstituteBVars(ss, bVars), s, md))
+        (SeqSubstituteIsDefinedOnLemma(ss, s.Keys);
+         SeqEval(ss, AdjustState(s), md) == 
+         SeqEval(SeqSubstitute(ss), s, md))
       decreases ss
     {
       if ss != [] {
-        SeqAdjustStateSubstituteBVarsLemma(ss[1..], s, bVars, md);
-        SeqSubstituteBVarsIsDefinedOnLemma(ss, bVars, s.Keys);
-        AdjustStateSubstituteBVarsLemma(s, ss[0], bVars, md);
+        SeqAdjustStateSubstituteLemma(ss[1..], s, md);
+        SeqSubstituteIsDefinedOnLemma(ss, s.Keys);
+        AdjustStateSubstituteLemma(s, ss[0], md);
       }
     }
 
 
-    lemma AdjustStateSubstituteBVarsLemma(s: State, e: Expr, bVars: set<Variable>, md: M.Model)
-      requires e.IsDefinedOn(incarnation.Keys + bVars)
-      requires incarnation.Values <= s.Keys + bVars
-      requires incarnation.Keys !! bVars
-      requires bVars <= s.Keys
-      ensures (SubstituteBVarsIsDefinedOnLemma(e, bVars, s.Keys);
-        e.Eval(s.Restrict(bVars) + AdjustStateBVars(s, bVars), md)) == SubstituteBVars(e, bVars).Eval(s, md)
+    lemma AdjustStateSubstituteLemma(s: State, e: Expr, md: M.Model)
+      requires e.IsDefinedOn(incarnation.Keys)
+      requires incarnation.Values <= s.Keys
+      ensures (SubstituteIsDefinedOnLemma(e, s.Keys);
+        e.Eval(AdjustState(s), md)) == Substitute(e).Eval(s, md)
       decreases e
     {
       match e
       case OperatorExpr(op, args) =>
-        SeqAdjustStateSubstituteBVarsLemma(args, s, bVars, md);
+        SeqAdjustStateSubstituteLemma(args, s, md);
       case FunctionCallExpr(func, args) =>
-        SeqAdjustStateSubstituteBVarsLemma(args, s, bVars, md);
-      case QuantifierExpr(univ, v, body) =>
-        assert body.FVars() <= e.FVars() + {v};
-        assert (incarnation - {v}).Values <= incarnation.Values;
-        DeleteVar({v}).SubstituteBVarsIsDefinedOnLemma(body, bVars + {v}, s.Keys + {v});
-        assert forall b: M.Any | md.HasType(b, v.typ.ToType()) ::
-          body.Eval((s.Restrict(bVars) + AdjustStateBVars(s, bVars)).UpdateAt(v, b), md) ==
-          DeleteVar({v}).SubstituteBVars(body, bVars + {v}).Eval(s.UpdateAt(v, b), md) by {
-          forall b: M.Any | md.HasType(b, v.typ.ToType()) 
-            ensures 
-              body.Eval((s.Restrict(bVars) + AdjustStateBVars(s, bVars)).UpdateAt(v, b), md) == 
-              DeleteVar({v}).SubstituteBVars(body, bVars + {v}).Eval(s.UpdateAt(v, b), md)
-            {
-              calc {
-                DeleteVar({v}).SubstituteBVars(body, bVars + {v}).Eval(s.UpdateAt(v, b), md);
-                == { DeleteVar({v}).AdjustStateSubstituteBVarsLemma(s.UpdateAt(v, b), body, bVars + {v}, md); }
-                body.Eval(s.UpdateAt(v, b).Restrict(bVars + {v}) + DeleteVar({v}).AdjustStateBVars(s.UpdateAt(v, b), bVars + {v}), md);
-                == { assert s.UpdateAt(v, b).Restrict(bVars + {v}) == s.Restrict(bVars).UpdateAt(v, b); }
-                body.Eval(s.Restrict(bVars).UpdateAt(v, b) + DeleteVar({v}).AdjustStateBVars(s.UpdateAt(v, b), bVars + {v}), md);
-                == { 
-                    assert DeleteVar({v}).AdjustState(s.UpdateAt(v, b)) == DeleteVar({v}).AdjustState(s);
-                    assume false;
-                 }
-                body.Eval((s.Restrict(bVars) + AdjustStateBVars(s, bVars)).UpdateAt(v, b), md);
-              }
-            }
-          ForallPush(s.Restrict(bVars) + AdjustStateBVars(s, bVars), s, body, DeleteVar({v}).SubstituteBVars(body, bVars + {v}), v, md);
+        SeqAdjustStateSubstituteLemma(args, s, md);
+      case QuantifierExpr(univ, v, body) => 
+        var v' := v.FreshVar(incarnation.Values);
+        SubstituteIsDefinedOnLemma(e, s.Keys);
+        forall b: M.Any | md.HasType(b, v.typ.ToType()) 
+          ensures body.Eval(AdjustState(s).UpdateAt(v, b), md) == UpdateIncarnation(v, v').Substitute(body).Eval(s.UpdateAt(v', b), md) {
+          calc {
+            UpdateIncarnation(v, v').Substitute(body).Eval(s.UpdateAt(v', b), md);
+            == { UpdateIncarnation(v, v').AdjustStateSubstituteLemma(s.UpdateAt(v', b), body, md); }
+            body.Eval(UpdateIncarnation(v, v').AdjustState(s.UpdateAt(v', b)), md);
+            == { body.EvalFVarsLemma(AdjustState(s).UpdateAt(v, b), UpdateIncarnation(v, v').AdjustState(s.UpdateAt(v', b)), md); }
+            body.Eval(AdjustState(s).UpdateAt(v, b), md);
+          }
         }
-      case QuantifierExpr(false, v, body) => assume false;
-        // SubstituteIdxIsDefinedOnLemma(e, i, |s|);
-        // assert forall b: M.Any | md.HasType(b, tp.ToType()) :: 
-        //   body.Eval((s[..i] + AdjustState(s[i..])).Update([b]), md) == 
-        //   SubstituteIdx(body, i + 1).Eval(s.Update([b]), md) by {
-        //   forall b: M.Any | md.HasType(b, tp.ToType()) 
-        //     ensures body.Eval((s[..i] + AdjustState(s[i..])).Update([b]), md) == SubstituteIdx(body, i + 1).Eval(s.Update([b]), md) {
-        //     assert ([b] + s)[..i+1] == [b] + s[..i];
-        //     assert ([b] + s)[i+1..] == s[i..];
-        //     assert ((s[..i] + AdjustState(s[i..])).Update([b])) == (([b] + s)[..i+1] + AdjustState(([b] + s)[i+1..]));
-        //     AdjustStateSubstituteIdxLemma([b] + s, body, i + 1, md);
-        //   }
-        // }
-        // ExistsPush(s[..i] + AdjustState(s[i..]), s, body, SubstituteIdx(body, i + 1), tp.ToType(), md);
       case BVar(v) => if v in incarnation.Keys { assert incarnation[v] in incarnation.Values; }
-      case LetExpr(v, rhs, body) => assume false;
-        // var b := SubstituteIdx(rhs, i).Eval(s, md) by {
-        //   SubstituteIdxIsDefinedOnLemma(rhs, i, |s|);
-        // }
-        // if b.Some? {
-        //   var b := b.value;
-        //   calc {
-        //     LetExpr(v, rhs, body).Eval(s[..i] + AdjustState(s[i..]), md);
-        //     ==
-        //     body.Eval((s[..i] + AdjustState(s[i..])).Update([rhs.Eval(s[..i] + AdjustState(s[i..]), md).value]), md);
-        //     == { SubstituteIdxIsDefinedOnLemma(rhs, i, |s|); }
-        //     body.Eval((s[..i] + AdjustState(s[i..])).Update([b]), md);
-        //     == { assert ([b] + s)[..i+1] == [b] + s[..i];
-        //         assert ([b] + s)[i+1..] == s[i..];
-        //         assert ((s[..i] + AdjustState(s[i..])).Update([b])) == (([b] + s)[..i+1] + AdjustState(([b] + s)[i+1..])); }
-        //     body.Eval(([b] + s)[..i+1] + AdjustState(([b] + s)[i+1..]), md);
-        //     == { AdjustStateSubstituteIdxLemma([b] + s, body, i + 1, md);
-        //         SubstituteIdxIsDefinedOnLemma(body, i + 1, |s| + 1); }
-        //     SubstituteIdx(body, i + 1).Eval(s.Update([b]), md);
-        //   }
-        // }
+      case LetExpr(v, rhs, body) =>
+        var v' := v.FreshVar(incarnation.Values);
+        var b := Substitute(rhs).Eval(s, md) by {
+          SubstituteIsDefinedOnLemma(rhs, s.Keys);
+        }
+        if b.Some? {
+          var b := b.value;
+          SubstituteIsDefinedOnLemma(e, s.Keys);
+          calc {
+            Substitute(e).Eval(s, md);
+            ==
+            LetExpr(v', Substitute(rhs), UpdateIncarnation(v, v').Substitute(body)).Eval(s, md);
+            ==
+            UpdateIncarnation(v, v').Substitute(body).Eval(s.UpdateAt(v', b), md);
+            == { UpdateIncarnation(v, v').AdjustStateSubstituteLemma(s.UpdateAt(v', b), body, md); }
+            body.Eval(UpdateIncarnation(v, v').AdjustState(s.UpdateAt(v', b)), md);
+            == { body.EvalFVarsLemma(AdjustState(s).UpdateAt(v, b), UpdateIncarnation(v, v').AdjustState(s.UpdateAt(v', b)), md); }
+            body.Eval(AdjustState(s).UpdateAt(v, b), md);
+          }
+        }
       case _  => 
     }
-
-//     lemma AdjustStateSubstituteEvalLemma(s: State, e: Expr, md: M.Model)
-//       requires e.IsDefinedOn(|incarnation|)
-//       requires forall ic <- incarnation :: ic < |s|
-//       ensures Substitute(e).IsDefinedOn(|s|)
-//       ensures e.Eval(AdjustState(s), md) == Substitute(e).Eval(s, md)
-//     {
-//       SubstituteIsDefinedOnLemma(e, |s|);
-//       AdjustStateSubstituteIdxLemma(s, e, 0, md);
-//       assert [] + AdjustState(s) == AdjustState(s);
-//     }
 
 //     lemma AdjustStateSubstituteLemma(s: State, e: Expr, md: M.Model)
 //       requires e.IsDefinedOn(|incarnation|)
@@ -336,38 +275,38 @@ module Context {
 //     }
 //   }
 
-    // lemma MkEntailmentLemma(e: Expr, st: State, md: M.Model)
-    //   requires e.IsDefinedOn(incarnation.Keys)
-    //   requires forall ic <- incarnation.Values :: ic in st.Keys
-    //   requires IsSatisfiedOn(st, md)
-    //   requires MkEntailment(e).Holds(md)
-    //   ensures e.HoldsOn(AdjustState(st), md)
-    // {
-    //   assert Implies(Conj(ctx), Substitute(e)).IsDefinedOn(|st|) by {
-    //     IsDefinedOnImpliesLemma(Conj(ctx), Substitute(e), st) by {
-    //       EvalConjLemma(ctx, st, md);
-    //       SubstituteIsDefinedOnLemma(e, st.Keys);
-    //     }
-    //   }
-    //   assert e.HoldsOn(AdjustState(st), md) by { 
-    //     calc {
-    //       e.HoldsOn(AdjustState(st), md);
-    //       { SubstituteIsDefinedOnLemma(e, st.Keys);
-    //         AdjustStateSubstituteLemma(st, e, md); }
-    //       Substitute(e).HoldsOn(st, md);
-    //       { EvalConjLemma(ctx, st, md);
-    //         AdjustStateSubstituteLemma(st, e, md);
-    //         HoldsOnImpliesLemma(Conj(ctx), Substitute(e), st, md); }
-    //       MkEntailment(e).Holds(md);
-    //     }
-    //   }
-    // }
+    lemma MkEntailmentLemma(e: Expr, st: State, md: M.Model)
+      requires e.IsDefinedOn(incarnation.Keys)
+      requires incarnation.Values <= st.Keys
+      requires IsSatisfiedOn(st, md)
+      requires MkEntailment(e).Holds(md)
+      ensures e.HoldsOn(AdjustState(st), md)
+    {
+      assert Implies(Conj(ctx), Substitute(e)).IsDefinedOn(st.Keys) by {
+        IsDefinedOnImpliesLemma(Conj(ctx), Substitute(e), st) by {
+          EvalConjLemma(ctx, st, md);
+          SubstituteIsDefinedOnLemma(e, st.Keys);
+        }
+      }
+      assert e.HoldsOn(AdjustState(st), md) by { 
+        calc {
+          e.HoldsOn(AdjustState(st), md);
+          { SubstituteIsDefinedOnLemma(e, st.Keys);
+            AdjustStateSubstituteLemma(st, e, md); }
+          Substitute(e).HoldsOn(st, md);
+          { EvalConjLemma(ctx, st, md);
+            AdjustStateSubstituteLemma(st, e, md);
+            HoldsOnImpliesLemma(Conj(ctx), Substitute(e), st, md); }
+          MkEntailment(e).Holds(md);
+        }
+      }
+    }
 
-//     function Add(e: Expr): Context
-//       requires e.IsDefinedOn(|incarnation|)
-//     {
-//       this.(ctx := ctx + [Substitute(e)])
-//     }
+    function Add(e: Expr): Context
+      requires e.IsDefinedOn(incarnation.Keys)
+    {
+      this.(ctx := ctx + [Substitute(e)])
+    }
 
 //     function SeqSubstitute(ss: seq<Expr>): seq<Expr>
 //       requires forall e <- ss :: e.IsDefinedOn(|incarnation|)
@@ -375,190 +314,191 @@ module Context {
 //       seq(|ss|, (i: nat) requires i < |ss| => Substitute(ss[i]))
 //     }
 
-//     lemma GetSeqSubstituteLemma(ss: seq<Expr>, e: Expr) returns (e': Expr) 
-//       requires forall e <- ss :: e.IsDefinedOn(|incarnation|)
-//       requires e in SeqSubstitute(ss)
-//       ensures e' in ss
-//       ensures Substitute(e') == e
-//     {
-//       e' := ss[Index(SeqSubstitute(ss), e)];
-//     }
+    lemma GetSeqSubstituteLemma(ss: seq<Expr>, e: Expr) returns (e': Expr) 
+      requires SeqExprFVars(ss) <= incarnation.Keys
+      requires e in SeqSubstitute(ss)
+      ensures e' in ss
+      ensures e'.IsDefinedOn(incarnation.Keys)
+      ensures Substitute(e') == e
+    {
+      if ss != [] {
+        if Substitute(ss[0]) == e {
+          e' := ss[0];
+        } else {
+          e' := GetSeqSubstituteLemma(ss[1..], e);
+        }
+      }
+    }
 
-//     function AddSeq(ss: seq<Expr>): Context
-//       requires forall e <- ss :: e.IsDefinedOn(|incarnation|)
-//     {
-//       this.(ctx := ctx + SeqSubstitute(ss))
-//     }
+    function AddSeq(ss: seq<Expr>): Context
+      requires SeqExprFVars(ss) <= incarnation.Keys
+    {
+      this.(ctx := ctx + SeqSubstitute(ss))
+    }
 
-//     function mkPreContext(proc: Procedure, args: CallArguments): Context
-//       requires Call(proc, args).ValidCalls()
-//       requires args.IsDefinedOn(|incarnation|)
-//       ensures |mkPreContext(proc, args).incarnation| == |args|
-//       ensures forall i <- mkPreContext(proc, args).incarnation :: i in incarnation
-//     {
-//       var incrPre := seq(|args|, (i: nat) requires i < |args| => 
-//         args.IsDefinedOnIn(args[i], |incarnation|);
-//         incarnation[args[i].v]);
-//       forall i <- incrPre 
-//         ensures i in incarnation
-//       {
-//         assert i == incrPre[Index(incrPre, i)];
-//         assert args[Index(incrPre, i)] in args;
-//         args.IsDefinedOnIn(args[Index(incrPre, i)], |incarnation|);
-//         assert i == incarnation[args[Index(incrPre, i)].v];
-//       }
-//       Context(ctx, incrPre)
-//     }
+    function mkPreContext(proc: Procedure, args: CallArguments): Context
+      requires Call(proc, args).ValidCalls()
+      requires args.IsDefinedOn(incarnation.Keys)
+      ensures mkPreContext(proc, args).incarnation.Keys == args.FVars()
+      ensures forall i <- mkPreContext(proc, args).incarnation.Values :: i in incarnation.Values
+    {
+      var incrPre := map v | v in args.FVars() :: incarnation[v];
+      Context(ctx, incrPre)
+    }
 
-//     lemma mkPreContextLemma(proc: Procedure, args: CallArguments, s: State)
-//       requires Call(proc, args).ValidCalls()
-//       requires args.IsDefinedOn(|incarnation|)
-//       requires forall i <- incarnation :: i < |s|
-//       ensures mkPreContext(proc, args).AdjustState(s) == args.Eval(AdjustState(s))
-//     {
-//       forall i | 0 <= i < |args|
-//         ensures (mkPreContext(proc, args).AdjustState(s))[i] == args.Eval(AdjustState(s))[i]
-//       {
-//         calc {
-//           (mkPreContext(proc, args).AdjustState(s))[i];
-//           == { args.IsDefinedOnIn(args[i], |incarnation|); 
-//                assert incarnation[args[i].v] in incarnation; }
-//           s[incarnation[args[i].v]];
-//           ==
-//           args.Eval(AdjustState(s))[i];
-//         }
-//       }
-//     }
+    lemma mkPreContextLemma(proc: Procedure, args: CallArguments, s: State)
+      requires Call(proc, args).ValidCalls()
+      requires args.IsDefinedOn(incarnation.Keys)
+      requires incarnation.Values <= s.Keys
+      ensures mkPreContext(proc, args).AdjustState(s) == args.Eval(AdjustState(s))
+    {
+      forall v | v in args.FVars()
+        ensures (mkPreContext(proc, args).AdjustState(s))[v] == args.Eval(AdjustState(s))[v]
+      {
+        assert incarnation[v] in incarnation.Values;
+        assert s[incarnation[v]] == args.Eval(AdjustState(s))[v];
+      }
+    }
 
-//     function mkPostContext(proc: Procedure, args: CallArguments, oldContext: Context): Context
-//       requires Call(proc, args).ValidCalls()
-//       requires args.IsDefinedOn(|incarnation|)
-//       requires args.IsDefinedOn(|oldContext.incarnation|)
-//       requires |oldContext.incarnation| >= args.NumInOutArgs()
-//       ensures |mkPostContext(proc, args, oldContext).incarnation| == |args| + args.NumInOutArgs()
-//     {
-//       var oldNum := args.NumInOutArgs();
-//       var incrPost: seq<Idx> := seq(|args|, (i: nat) requires i < |args| => 
-//         args.IsDefinedOnIn(args[i], |incarnation|);
-//         incarnation[args[i].v]); 
-//       var incrPostOld: seq<Idx> := seq(args.NumInOutArgs(), (i: nat) requires i < args.NumInOutArgs() => 
-//         args.InOutArgsLemma(args.InOutArgs()[i]); 
-//         args.IsDefinedOnIn(InOutArgument(args.InOutArgs()[i]), |oldContext.incarnation|);
-//         oldContext.incarnation[args.InOutArgs()[i]]);
-//       Context(ctx, incrPost + incrPostOld)
-//     }
+    function mkPostContext(proc: Procedure, args: CallArguments/*, oldContext: Context*/): Context
+      requires Call(proc, args).ValidCalls()
+      requires args.IsDefinedOn(incarnation.Keys)
+      // requires args.IsDefinedOn(oldContext.incarnation.Keys)
+      // requires |oldContext.incarnation| >= args.NumInOutArgs()
+      ensures mkPostContext(proc, args/*, oldContext*/).incarnation.Keys == args.FVars() /*+ args.NumInOutArgs()*/
+    {
+      // var oldNum := args.NumInOutArgs();
+      var incrPost: map<Variable, Variable> := map v | v in args.FVars() :: incarnation[v];
+      // var incrPostOld: seq<Idx> := seq(args.NumInOutArgs(), (i: nat) requires i < args.NumInOutArgs() => 
+      //   args.InOutArgsLemma(args.InOutArgs()[i]); 
+      //   args.IsDefinedOnIn(InOutArgument(args.InOutArgs()[i]), |oldContext.incarnation|);
+      //   oldContext.incarnation[args.InOutArgs()[i]]);
+      Context(ctx, incrPost /*+ incrPostOld*/)
+    }
 
-//     lemma mkPostContextIncrSubsetLemma(proc: Procedure, args: CallArguments, oldContext: Context, i: nat)
-//       requires Call(proc, args).ValidCalls()
-//       requires args.IsDefinedOn(|incarnation|)
-//       requires args.IsDefinedOn(|oldContext.incarnation|)
-//       requires |oldContext.incarnation| >= args.NumInOutArgs()
-//       requires i in mkPostContext(proc, args, oldContext).incarnation
-//       ensures i in oldContext.incarnation || i in incarnation
-//     {
-//       var oldNum := args.NumInOutArgs();
-//       var incrPost: seq<Idx> := seq(|args|, (i: nat) requires i < |args| => 
-//         args.IsDefinedOnIn(args[i], |incarnation|);
-//         incarnation[args[i].v]); 
-//       var incrPostOld: seq<Idx> := seq(args.NumInOutArgs(), (i: nat) requires i < args.NumInOutArgs() => 
-//         args.InOutArgsLemma(args.InOutArgs()[i]); 
-//         args.IsDefinedOnIn(InOutArgument(args.InOutArgs()[i]), |oldContext.incarnation|);
-//         oldContext.incarnation[args.InOutArgs()[i]]);
-//       assert incrPost + incrPostOld == mkPostContext(proc, args, oldContext).incarnation;
-//       assert i in incrPost + incrPostOld;
-//       if i in incrPost {
-//         assert i == incrPost[Index(incrPost, i)];
-//         args.IsDefinedOnIn(args[Index(incrPost, i)], |incarnation|);
-//         assert i == incarnation[args[Index(incrPost, i)].v];
-//       } else {
-//         assert i in incrPostOld;
-//         assert i == incrPostOld[Index(incrPostOld, i)];
-//         args.InOutArgsLemma(args.InOutArgs()[Index(incrPostOld, i)]);
-//         args.IsDefinedOnIn(InOutArgument(args.InOutArgs()[Index(incrPostOld, i)]), |oldContext.incarnation|);
-//         assert i == oldContext.incarnation[args.InOutArgs()[Index(incrPostOld, i)]];
-//       }
-//     }
+    lemma mkPostContextIncrSubsetLemma(proc: Procedure, args: CallArguments,/* oldContext: Context,*/ v: Variable)
+      requires Call(proc, args).ValidCalls()
+      requires args.IsDefinedOn(incarnation.Keys)
+      // requires args.IsDefinedOn(|oldContext.incarnation|)
+      // requires |oldContext.incarnation| >= args.NumInOutArgs()
+      requires v in mkPostContext(proc, args/*, oldContext*/).incarnation.Values
+      ensures /*i in oldContext.incarnation ||*/ v in incarnation.Values
+    {
+      // var oldNum := args.NumInOutArgs();
+      // var incrPost: seq<Idx> := seq(|args|, (i: nat) requires i < |args| => 
+      //   args.IsDefinedOnIn(args[i], |incarnation|);
+      //   incarnation[args[i].v]); 
+      // var incrPostOld: seq<Idx> := seq(args.NumInOutArgs(), (i: nat) requires i < args.NumInOutArgs() => 
+      //   args.InOutArgsLemma(args.InOutArgs()[i]); 
+      //   args.IsDefinedOnIn(InOutArgument(args.InOutArgs()[i]), |oldContext.incarnation|);
+      //   oldContext.incarnation[args.InOutArgs()[i]]);
+      // assert incrPost + incrPostOld == mkPostContext(proc, args, oldContext).incarnation;
+      // assert i in incrPost + incrPostOld;
+      // if i in incrPost {
+      //   assert i == incrPost[Index(incrPost, i)];
+      //   args.IsDefinedOnIn(args[Index(incrPost, i)], |incarnation|);
+      //   assert i == incarnation[args[Index(incrPost, i)].v];
+      // } else {
+      //   assert i in incrPostOld;
+      //   assert i == incrPostOld[Index(incrPostOld, i)];
+      //   args.InOutArgsLemma(args.InOutArgs()[Index(incrPostOld, i)]);
+      //   args.IsDefinedOnIn(InOutArgument(args.InOutArgs()[Index(incrPostOld, i)]), |oldContext.incarnation|);
+      //   assert i == oldContext.incarnation[args.InOutArgs()[Index(incrPostOld, i)]];
+      // }
+    }
 
-//     method AddEq(v: Idx, e: Expr) returns (ghost vNew: Idx, context: Context)
-//       requires v < |incarnation|
-//       requires e.IsDefinedOn(|incarnation|)
-//       ensures |incarnation| == |context.incarnation|
-//       ensures ctx + [Eq(BVar(vNew), Substitute(e))] == context.ctx
-//       ensures incarnation[v := vNew] == context.incarnation
-//       ensures forall i <- incarnation :: i < vNew 
-//       ensures forall c <- ctx :: c.Depth() < vNew
-//       ensures SeqMax(incarnation) < vNew
-//       ensures SeqExprDepth(ctx) < vNew
-//       // ensures 
-//     {
-//       var v' := FreshIdx();
-//       var ctx' := ctx + [Eq(BVar(v'), Substitute(e))];
-//       var incarnation' := incarnation[v := v'];
-//       context := Context(ctx', incarnation');
-//       vNew := v';
-//     }
+    method AddEq(v: Variable, e: Expr) returns (ghost vNew: Variable, context: Context)
+      requires v in incarnation.Keys
+      requires e.IsDefinedOn(incarnation.Keys)
+      ensures incarnation.Keys == context.incarnation.Keys
+      ensures ctx + [Eq(BVar(vNew), Substitute(e))] == context.ctx
+      ensures incarnation[v := vNew] == context.incarnation
+      // ensures forall i <- incarnation.Values :: i < vNew 
+      ensures forall c <- ctx :: vNew !in c.FVars()
+      ensures vNew !in incarnation.Values
+      ensures vNew !in SeqExprFVars(ctx)
+      // ensures 
+    {
+      var v' := FreshVar(v.typ);
+      var ctx' := ctx + [Eq(BVar(v'), Substitute(e))];
+      var incarnation' := incarnation[v := v'];
+      context := Context(ctx', incarnation');
+      vNew := v';
+    }
 
-//     method AddVarSet(vars: set<Idx>) returns (ghost vNew: Idx, context: Context)
-//       requires forall v <- vars :: v < |incarnation|
-//       ensures context.ctx         == ctx
-//       ensures |context.incarnation| == |incarnation|
-//       ensures forall i: nat :: i in vars ==> context.incarnation[i] == vNew + i
-//       ensures vNew > SeqMax(incarnation)
-//       ensures forall c <- ctx :: c.Depth() < vNew
-//       ensures SeqExprDepth(ctx) < vNew
-//       ensures forall i: nat :: i !in vars && i < |incarnation| ==> context.incarnation[i] == incarnation[i]
-//       ensures forall i <- context.incarnation :: i <= vNew + Max'(vars)
-//     {
-//       var vars' := vars; 
-//       var incr' := incarnation;
-//       var v' := FreshIdx();
-//       vNew := v';
-//       while vars' != {}
-//         invariant |incr'| == |incarnation|
-//         invariant vars' <= vars
-//         invariant forall i: nat :: i in vars - vars' ==> incr'[i] == vNew + i
-//         invariant forall i: nat :: i !in vars - vars' && i < |incarnation| ==> incr'[i] == incarnation[i]
-//         invariant forall i: nat :: i < |incarnation| ==> incr'[i] <= vNew + Max'(vars)
-//       {
-//         var v :| v in vars';
-//         vars' := vars' - {v};
-//         incr' := incr'[v := v' + v];
-//       }
-//       context := Context(ctx, incr');
-//     }
+    method AddVarSet(vars: set<Variable>) returns (ghost vsNew: map<Variable, Variable>, context: Context)
+      // requires vars <= incarnation.Keys
+      ensures vsNew.Values == vars
+      ensures context.ctx         == ctx
+      ensures context.incarnation.Keys == incarnation.Keys + vars
+      ensures forall v <- vars :: context.incarnation[v] in vsNew.Keys && vsNew[context.incarnation[v]] == v
+      ensures vsNew.Keys !! incarnation.Values
+      ensures forall c <- ctx :: c.FVars() !! vsNew.Keys
+      ensures SeqExprFVars(ctx) !! vsNew.Keys
+      ensures forall v <- incarnation.Keys :: v !in vars ==> context.incarnation[v] == incarnation[v]
+      ensures context.incarnation.Values <= vsNew.Keys + incarnation.Values
+    {
+      var vars' := vars; 
+      var incr' := incarnation;
+      var vs: map<Variable, Variable> := map[];
+      // vNew := v';
+      while vars' != {}
+        invariant incr'.Keys == incarnation.Keys + (vars - vars')
+        invariant vars' <= vars
+        invariant forall v <- vars - vars' :: incr'[v] in vs.Keys && vs[incr'[v]] == v
+        invariant vs.Keys !! incarnation.Values
+        invariant forall v <- incarnation.Keys :: v !in vars - vars' ==> incr'[v] == incarnation[v]
+        invariant incr'.Values <= vs.Keys + incarnation.Values
+        invariant forall c <- ctx :: c.FVars() !! vs.Keys
+        invariant SeqExprFVars(ctx) !! vs.Keys
+        invariant vs.Values == vars - vars'
+      {
+        var v :| v in vars';
+        vars' := vars' - {v};
+        var v' := FreshVarSet(v.typ, vs.Keys);
+        assert vs[v' := v].Values == vs.Values + {v} by {
+          assert vs[v' := v] == vs + map[v' := v];
+        }
+        vs := vs[v' := v];
+        incr' := incr'[v := v'];
+      }
+      vsNew := vs;
+      context := Context(ctx, incr');
+    }
 
-//     function Delete(n: nat): Context
-//       requires n <= |incarnation|
-//     {
-//       Context(ctx, incarnation[n..])
-//     }
+    function Delete(vars: set<Variable>): Context
+      requires vars <= incarnation.Keys
+    {
+      Context(ctx, incarnation - vars)
+    }
       
 
-//     method AddVars(n: nat) returns (ghost vNew: Idx, context: Context)
-//       // ensures incarnation <= AddVars(n).incarnation 
-//       ensures context.ctx         == ctx
-//       ensures |context.incarnation| == |incarnation| + n
-//       ensures forall i: nat :: i < n ==> context.incarnation[i] == vNew + i
-//       ensures forall i: nat :: n <= i < |incarnation| + n ==> context.incarnation[i] == incarnation[i - n]
-//       ensures forall c <- ctx :: c.Depth() < vNew
-//       ensures SeqMax(incarnation) < vNew
-//       ensures SeqExprDepth(ctx) < vNew
-//     {
-//       var v := FreshIdx();
-//       var addOn := seq(n, (i: nat) => v + i);
-//       context := Context(ctx, addOn + incarnation);
-//       vNew := v;
-//     }
+    // method AddVars(n: nat) returns (ghost vNew: Idx, context: Context)
+    //   // ensures incarnation <= AddVars(n).incarnation 
+    //   ensures context.ctx         == ctx
+    //   ensures |context.incarnation| == |incarnation| + n
+    //   ensures forall i: nat :: i < n ==> context.incarnation[i] == vNew + i
+    //   ensures forall i: nat :: n <= i < |incarnation| + n ==> context.incarnation[i] == incarnation[i - n]
+    //   ensures forall c <- ctx :: c.Depth() < vNew
+    //   ensures SeqMax(incarnation) < vNew
+    //   ensures SeqExprDepth(ctx) < vNew
+    // {
+    //   var v := FreshIdx();
+    //   var addOn := seq(n, (i: nat) => v + i);
+    //   context := Context(ctx, addOn + incarnation);
+    //   vNew := v;
+    // }
 
 //     // lemma SubstituteIdxIsDefinedOnLemmaOperator
+  }
 
-//   function mkInitialContext(proc: Procedure): Context
-//   {
-//     var incr := seq(|proc.Parameters|, (i: nat) => i);
-//     var incrOld := seq(proc.NumInOutArgs(), (i: nat) requires i < proc.NumInOutArgs() => 
-//       proc.InOutVarsIdxs()[i]);
-//     Context(proc.Pre, incr + incrOld)
-//   }
+  function mkInitialContext(proc: Procedure): Context
+  {
+    var incr := map v | v in proc.ParametersKeys() :: v;
+    // var incrOld := seq(proc.NumInOutArgs(), (i: nat) requires i < proc.NumInOutArgs() => 
+    //   proc.InOutVarsIdxs()[i]);
+    Context(proc.Pre, incr /*+ incrOld*/)
+  }
 
 //   lemma mkInitialContextLemma(proc: Procedure, i: nat)
 //     requires i in mkInitialContext(proc).incarnation
@@ -571,5 +511,5 @@ module Context {
 //       assert i == proc.InOutVarsIdxs()[Index(incrOld, i)];
 //       proc.InOutVarsIdxsLemma(proc.Parameters, 0, Index(incrOld, i));
 //     }
-  }
+  // }
 }
